

AARHUS UNIVERSITY

COMPUTER-SCIENCE

INTRODUCTION TO PROBABILITY AND STATISTICS

Handin 4

Author

Søren M. DAMSGAARD

Student number

202309814

September 25, 2025



Let $0 < p < 1$ and $X \approx \text{Geometric}(p)$.

Calculate The cumulative distribution function (CDF) $F_X(x) = P(X \leq x)$ for all $x = 1, 2, 3, \dots$

Show that X has the 'lack of memory' property, i.e.

$$P(X > m + k | X > m) = P(X > k) \text{ for all } k, m = 1, 2, 3, \dots \quad (1)$$

Finding the CDF (Dora's solution)

The CDF is essentially the sum of all the probabilities up to and including x for discrete variables.

This means that we can express it as:

$$F_X(x) = P(X \leq x) = \sum_{i=1}^x P(X = i) \quad \text{for } x = 1, 2, 3, \dots \quad (2)$$

From Def 3.5 [1] we know that the PMF of a geometric distribution is:

$$P(X = i) = (1 - p)^{i-1}p \quad (3)$$

This means that we can rewrite the CDF as:

$$F_X(x) = \sum_{i=1}^x (1 - p)^{i-1}p \quad (4)$$

Move the constant out of the summation:

$$F_X(x) = p \sum_{i=1}^x (1 - p)^{i-1} \quad (5)$$

We will now show that the current summation is a geometric series.

A geometric series is defined as:

$$a + ax + ax^2 + ax^3 + \dots + ax^{n-1} = \sum_{k=0}^{n-1} ax^k = a \frac{1 - x^n}{1 - x} \quad (6)$$

from example 1.12 equation 1.3 [1].

We can see that our summation is a geometric series with $a = 1$, $x = (1 - p)$ and $n = x$.

This means that we can rewrite the CDF as:

$$F_X(x) = p \cdot \frac{1 - (1 - p)^x}{1 - (1 - p)} \quad (7)$$

which simplifies to:

$$F_X(x) = 1 - (1 - p)^x \quad (8)$$

Note that it's important when we use the geometric series we, it has to start at index 0, so we had to re

Show X has dementia (lack of memory property)

Reiterating equation(1)

$$P(X > m + k | X > m) = P(X > k) \text{ for all } k, m = 1, 2, 3, \dots$$

We use the definition of conditional probability from chapter 1.4 [1] to do legal crime:

$$P(A|B) = \frac{P(A \cap B)}{P(B)} \quad (9)$$

We can then rewrite the right side of equation(1) as:

$$P(X > m + k | X > m) = \frac{P((X > m + k) \cap (X > m))}{P(X > m)} = \frac{P(X > m + k)}{P(X > m)} \quad (10)$$

We note here that $P((X > m + k) \cap (X > m)) = P(X > m + k)$ since $X > m + k \implies X > m$.

We can now use the CDF we found earlier to express $P(X > x)$ using the complement, like from example 3.10 [1]:

$$P(X > x) = 1 - P(X \leq x) = 1 - F_X(x) \quad (11)$$

We can then take equation(10) and throw our new math at it like Kobe Bryant on January 22, 2006 (60 points on 50 shots):

$$P(X > m + k | X > m) = \frac{1 - F_X(m + k)}{1 - F_X(m)} \quad (12)$$

We can then insert the value of the CDF:

$$P(X > m + k | X > m) = \frac{1 - (1 - (1 - p)^{m+k})}{1 - (1 - (1 - p)^m)} \quad (13)$$

which we can beautify a little bit by removing the negative vibes:

$$P(X > m + k | X > m) = \frac{(1 - p)^{m+k}}{(1 - p)^m} \quad (14)$$

And as a finishing touch we will put the crown on it by simplifying the fraction even further:

$$P(X > m + k | X > m) = (1 - p)^k \quad (15)$$

Now we can see that the right side of equation(1) is:

$$P(X > k) = 1 - F_X(k) = 1 - (1 - (1 - p)^k) = (1 - p)^k \quad (16)$$

References

- [1] Hossein Pishro-Nik. *Introduction to Probability ,Statistics and Random Processes*. Kappa Research, LLC, 2014.